erasure/theories/EInversion.v
@@ -20,31 +20,6 @@ Local Existing Instance default_checker_flags.
 
 (** ** Inversion on eval *)
 
-Lemma type_Case_inv (Σ : global_env_ext) (hΣ : wf Σ.1) Γ ind npar p c brs T :
-  Σ;;; Γ |- PCUICAst.tCase (ind, npar) p c brs : T ->
-  { '(u, args, mdecl, idecl, pty, indctx, pctx, ps, btys) : _ &
-         (PCUICTyping.declared_inductive (fst Σ) mdecl ind idecl) *
-         (PCUICAst.ind_npars mdecl = npar) *
-         let pars := firstn npar args in
-         (Σ;;; Γ |- p : pty) *
-         (types_of_case ind mdecl idecl pars u p pty = Some (indctx, pctx, ps, btys)) *
-         (check_correct_arity (global_ext_constraints Σ) idecl ind u indctx pars pctx) *
-         (existsb (leb_sort_family (universe_family ps)) (PCUICAst.ind_kelim idecl)) *
-         (Σ;;; Γ |- c : PCUICAst.mkApps (tInd ind u) args) *
-         (All2 (fun x y : nat * PCUICAst.term => ((fst x = fst y) * (Σ;;; Γ |- snd x : snd y)) * (Σ ;;; Γ |- snd y : tSort ps)) brs btys) *
-         (Σ ;;; Γ |- PCUICAst.mkApps p (skipn npar args ++ [c])  <= T)}%type.
-Proof.
-  intros. dependent induction X.
-  - unshelve eexists.
-    + repeat refine (_,_). all:shelve.
-    + cbn. subst pars. intuition eauto.
-  - edestruct (IHX hΣ _ _ _ _ _ eq_refl) as [ [[[[[[[[]]]]]]]] ].
-    repeat match goal with [ H : _ * _ |- _ ] => destruct H end.
-    unshelve eexists.
-    + repeat refine (_, _). all:shelve.
-    + cbn. intuition eauto.
-      all: eapply PCUICConversion.cumul_trans; eauto.
-Qed.
 
 Notation type_Construct_inv := PCUICInversion.inversion_Construct.
 Notation type_tFix_inv := PCUICInversion.inversion_Fix.
